Split well-formedness in two.

theories/language/well_formed.v
@@ -15,50 +15,88 @@ Definition val_well_formed prog v :=
       True
   end.
 
-Fixpoint expr_well_formed prog lvl e :=
+Fixpoint expr_well_formed prog e :=
   match e with
   | Val v =>
       val_well_formed prog v
-  | Var x =>
-      x < lvl
+  | Var _ =>
+      True
   | Let e1 e2 =>
-      expr_well_formed prog lvl e1 ∧
-      expr_well_formed prog (S lvl) e2
+      expr_well_formed prog e1 ∧
+      expr_well_formed prog e2
   | Call e1 e2 =>
-      expr_well_formed prog lvl e1 ∧
-      expr_well_formed prog lvl e2
+      expr_well_formed prog e1 ∧
+      expr_well_formed prog e2
   | Unop _ e =>
-      expr_well_formed prog lvl e
+      expr_well_formed prog e
   | Binop _ e1 e2 =>
-      expr_well_formed prog lvl e1 ∧
-      expr_well_formed prog lvl e2
+      expr_well_formed prog e1 ∧
+      expr_well_formed prog e2
   | If e0 e1 e2 =>
-      expr_well_formed prog lvl e0 ∧
-      expr_well_formed prog lvl e1 ∧
-      expr_well_formed prog lvl e2
+      expr_well_formed prog e0 ∧
+      expr_well_formed prog e1 ∧
+      expr_well_formed prog e2
   | Constr constr e1 e2 =>
-      expr_well_formed prog lvl e1 ∧
-      expr_well_formed prog lvl e2
+      expr_well_formed prog e1 ∧
+      expr_well_formed prog e2
   | ConstrDet _ _ _ =>
       False
   | Load e1 e2 =>
-      expr_well_formed prog lvl e1 ∧
-      expr_well_formed prog lvl e2
+      expr_well_formed prog e1 ∧
+      expr_well_formed prog e2
   | Store e1 e2 e3 =>
-      expr_well_formed prog lvl e1 ∧
-      expr_well_formed prog lvl e2 ∧
-      expr_well_formed prog lvl e3
+      expr_well_formed prog e1 ∧
+      expr_well_formed prog e2 ∧
+      expr_well_formed prog e3
   end.
 
-Definition expr_well_formed' prog e :=
-  ∃ lvl, expr_well_formed prog lvl e.
+Fixpoint expr_closed lvl e :=
+  match e with
+  | Val _ =>
+      True
+  | Var x =>
+      x < lvl
+  | Let e1 e2 =>
+      expr_closed lvl e1 ∧
+      expr_closed (S lvl) e2
+  | Call e1 e2 =>
+      expr_closed lvl e1 ∧
+      expr_closed lvl e2
+  | Unop _ e =>
+      expr_closed lvl e
+  | Binop _ e1 e2 =>
+      expr_closed lvl e1 ∧
+      expr_closed lvl e2
+  | If e0 e1 e2 =>
+      expr_closed lvl e0 ∧
+      expr_closed lvl e1 ∧
+      expr_closed lvl e2
+  | Constr constr e1 e2 =>
+      expr_closed lvl e1 ∧
+      expr_closed lvl e2
+  | ConstrDet _ _ _ =>
+      False
+  | Load e1 e2 =>
+      expr_closed lvl e1 ∧
+      expr_closed lvl e2
+  | Store e1 e2 e3 =>
+      expr_closed lvl e1 ∧
+      expr_closed lvl e2 ∧
+      expr_closed lvl e3
+  end.
 
 Definition program_well_formed prog :=
-  map_Forall (λ _, expr_well_formed prog 1) prog.
+  map_Forall (λ _, expr_well_formed prog) prog.
 
-Lemma subst_expr_well_formed ς1 ς2 prog lvl e :
+Definition program_closed prog :=
+  map_Forall (λ _, expr_closed 1) prog.
+
+Definition program_valid prog :=
+  program_well_formed prog ∧ program_closed prog.
+
+Lemma subst_expr_closed ς1 ς2 lvl e :
   (∀ x, x < lvl → ς1 x = ς2 x) →
-  expr_well_formed prog lvl e →
+  expr_closed lvl e →
   e.[ς1] = e.[ς2].
 Proof.
   revert ς1 ς2 lvl. induction e as
@@ -74,114 +112,113 @@ Proof.
     | e1 IHe1 e2 IHe2
     | e1 IHe1 e2 IHe2 e3 IHe3
     ];
-    intros ς1 ς2 lvl Hς Hwf;
+    intros ς1 ς2 lvl Hς Hclosed;
     asimpl;
     try (f_equal; naive_solver).
   f_equal; first naive_solver.
   eapply IHe2; last naive_solver.
   intros x Hx. destruct x; first done. asimpl. f_equal. naive_solver lia.
 Qed.
-Lemma subst_expr_well_formed_0 ς1 ς2 prog e :
-  expr_well_formed prog 0 e →
+Lemma subst_expr_closed_0 ς1 ς2 e :
+  expr_closed 0 e →
   e.[ς1] = e.[ς2].
 Proof.
-  intros Hwf.
-  eapply subst_expr_well_formed; last done.
+  intros Hclosed.
+  eapply subst_expr_closed; last done.
   lia.
 Qed.
-Lemma subst_expr_well_formed_1 ς1 ς2 prog e :
+Lemma subst_expr_closed_1 ς1 ς2 e :
   ς1 0 = ς2 0 →
-  expr_well_formed prog 1 e →
+  expr_closed 1 e →
   e.[ς1] = e.[ς2].
 Proof.
-  intros Hς Hwf.
-  eapply subst_expr_well_formed; last done.
+  intros Hς Hclosed.
+  eapply subst_expr_closed; last done.
   setoid_rewrite Nat.lt_1_r. naive_solver.
 Qed.
-Lemma subst_expr_well_formed_1' ς1 ς2 v prog e :
-  expr_well_formed prog 1 e →
+Lemma subst_expr_closed_1' ς1 ς2 v e :
+  expr_closed 1 e →
   e.[v .: ς1] = e.[v .: ς2].
 Proof.
-  apply subst_expr_well_formed_1. done.
+  apply subst_expr_closed_1. done.
 Qed.
-Lemma subst_program_well_formed ς1 ς2 prog func e :
+
+Lemma subst_program_closed ς1 ς2 prog func e :
   ς1 0 = ς2 0 →
-  program_well_formed prog →
+  program_closed prog →
   prog !! func = Some e →
   e.[ς1] = e.[ς2].
 Proof.
   intros Hσ Hwf Hlookup.
-  eapply subst_expr_well_formed_1; first done.
-  pose proof (map_Forall_lookup_1 _ _ _ _ Hwf Hlookup). eauto.
+  eapply subst_expr_closed_1; first done.
+  eapply map_Forall_lookup_1 in Hwf; naive_solver.
 Qed.
-Lemma subst_program_well_formed' ς1 ς2 v prog func e :
-  program_well_formed prog →
+Lemma subst_program_closed' ς1 ς2 v prog func e :
+  program_closed prog →
   prog !! func = Some e →
   e.[v .: ς1] = e.[v .: ς2].
 Proof.
-  apply subst_program_well_formed. done.
+  apply subst_program_closed. done.
 Qed.
 
-Lemma expr_well_formed_le prog lvl1 lvl2 e :
+Lemma expr_closed_le lvl1 lvl2 e :
   lvl1 ≤ lvl2 →
-  expr_well_formed prog lvl1 e →
-  expr_well_formed prog lvl2 e.
+  expr_closed lvl1 e →
+  expr_closed lvl2 e.
 Proof.
   revert lvl1 lvl2. elim e; try naive_solver lia.
-  intros e1 IH1 e2 IH2 lvl1 lvl2 Hlvl (Hwf1 & Hwf2).
+  intros e1 IH1 e2 IH2 lvl1 lvl2 Hlvl (Hclosed1 & Hclosed2).
   split; first naive_solver. eapply IH2; last done. lia.
 Qed.
 
-Lemma expr_well_formed_upn_subst_val n v prog lvl e :
+Lemma expr_closed_upn_subst_val n v lvl e :
   n < lvl →
-  val_well_formed prog v →
-  expr_well_formed prog lvl e →
-  expr_well_formed prog (lvl - 1) e.[upn n (Val v .: ids)].
+  expr_closed lvl e →
+  expr_closed (lvl - 1) e.[upn n (Val v .: ids)].
 Proof.
   revert n lvl. induction e; intros n lvl; try naive_solver; simpl.
-  - intros Hn Hv Hx.
+  - intros Hn Hx.
     destruct (Nat.lt_ge_cases x n) as [Hx' | (dx & ->)%Nat.le_sum].
     + rewrite upn_lt //=. lia.
     + rewrite upn_ge; first lia.
       rewrite Nat.sub_add'. destruct dx; first done. simpl. lia.
-  - intros Hn Hv (Hwf1 & Hwf2). split; first naive_solver.
+  - intros Hn (Hclosed1 & Hclosed2). split; first naive_solver.
     rewrite fold_up_upn.
     destruct lvl; first lia.
     rewrite /= Nat.sub_0_r -(Nat.pred_succ (S lvl)) -Nat.sub_1_r.
     auto with lia.
 Qed.
-Lemma expr_well_formed_subst_val prog lvl e v :
-  val_well_formed prog v →
-  expr_well_formed prog lvl e →
-  expr_well_formed prog (lvl - 1) e.[Val v/].
+Lemma expr_closed_subst_val lvl e v :
+  expr_closed lvl e →
+  expr_closed (lvl - 1) e.[Val v/].
 Proof.
   destruct lvl.
-  - intros Hv Hwf%(expr_well_formed_le _ _ 1)%(expr_well_formed_upn_subst_val 0 v); naive_solver lia.
-  - apply (expr_well_formed_upn_subst_val 0). lia.
+  - intros Hclosed%(expr_closed_le _ 1)%(expr_closed_upn_subst_val 0 v); naive_solver lia.
+  - apply (expr_closed_upn_subst_val 0). lia.
 Qed.
 
-Lemma expr_well_formed_ren ξ n prog lvl e :
+Lemma expr_closed_ren ξ n lvl e :
   (∀ x, ξ x ≤ x + n) →
-  expr_well_formed prog lvl e →
-  expr_well_formed prog (lvl + n) e.[ren ξ].
+  expr_closed lvl e →
+  expr_closed (lvl + n) e.[ren ξ].
 Proof.
   revert lvl ξ n. elim e; try naive_solver lia.
-  - intros x lvl ξ n Hξ Hwf.
+  - intros x lvl ξ n Hξ Hclosed.
     eapply (Nat.le_lt_trans _ (x + n)); naive_solver lia.
-  - intros e1 IH1 e2 IH2 lvl ξ n Hξ (Hwf1 & Hwf2).
+  - intros e1 IH1 e2 IH2 lvl ξ n Hξ (Hclosed1 & Hclosed2).
     split; first naive_solver.
     asimpl. rewrite -Nat.add_succ_l. apply IH2; last done.
     intros []; simpl; [lia | rewrite -Nat.succ_le_mono //].
 Qed.
-Lemma expr_well_formed_lift n prog lvl e :
-  expr_well_formed prog lvl e →
-  expr_well_formed prog (lvl + n) e.[ren (+n)].
+Lemma expr_closed_lift n lvl e :
+  expr_closed lvl e →
+  expr_closed (lvl + n) e.[ren (+n)].
 Proof.
-  apply expr_well_formed_ren. naive_solver lia.
+  apply expr_closed_ren. naive_solver lia.
 Qed.
-Lemma expr_well_formed_lift1 prog lvl e :
-  expr_well_formed prog lvl e →
-  expr_well_formed prog (S lvl) e.[ren (+1)].
+Lemma expr_closed_lift1 lvl e :
+  expr_closed lvl e →
+  expr_closed (S lvl) e.[ren (+1)].
 Proof.
-  rewrite -Nat.add_1_r. apply expr_well_formed_lift.
+  rewrite -Nat.add_1_r. apply expr_closed_lift.
 Qed.
