theories/tmc/properties.v
@@ -9,138 +9,134 @@ From simuliris.language Require Import
 From simuliris.tmc Require Export
   definition.
 
-Lemma tmc_dir_refl ξ e :
-  tmc_dir ξ e e.
-Proof.
-  induction e; eauto with tmc.
-Qed.
-#[export] Hint Resolve tmc_dir_refl : tmc.
+Section tmc.
+  Context (ξ : gmap function function).
 
-Lemma tmc_subst ξ :
-  ( ∀ eₛ eₜ,
+  Lemma tmc_dir_refl e :
+    tmc_dir ξ e e.
+  Proof.
+    induction e; eauto with tmc.
+  Qed.
+
+  Lemma tmc_subst :
+    ( ∀ eₛ eₜ,
+      tmc_dir ξ eₛ eₜ →
+      ∀ eₛ' eₜ' ς,
+      eₛ' = eₛ.[ς] →
+      eₜ' = eₜ.[ς] →
+      tmc_dir ξ eₛ' eₜ'
+    ) ∧ (
+      ∀ dst idx eₛ eₜ,
+      tmc_dps ξ dst idx eₛ eₜ →
+      ∀ dst' idx' eₛ' eₜ' ς,
+      dst' = dst.[ς] →
+      idx' = idx.[ς] →
+      eₛ' = eₛ.[ς] →
+      eₜ' = eₜ.[ς] →
+      tmc_dps ξ dst' idx' eₛ' eₜ'
+    ).
+  Proof.
+    apply tmc_ind; solve
+    [ intros; simplify; eauto using tmc_dir_refl
+    | intros * ? ? ? IHdps **; simplify;
+      econstructor; try naive_solver; try eapply IHdps with (up ς); autosubst
+    ].
+  Qed.
+  Lemma tmc_dir_subst ς eₛ eₛ' eₜ eₜ' :
     tmc_dir ξ eₛ eₜ →
-    ∀ eₛ' eₜ' ς,
     eₛ' = eₛ.[ς] →
     eₜ' = eₜ.[ς] →
-    tmc_dir ξ eₛ' eₜ'
-  ) ∧ (
-    ∀ dst idx eₛ eₜ,
+    tmc_dir ξ eₛ' eₜ'.
+  Proof.
+    eauto using (proj1 tmc_subst).
+  Qed.
+  Lemma tmc_dps_subst ς dst dst' idx idx' eₛ eₛ' eₜ eₜ' :
     tmc_dps ξ dst idx eₛ eₜ →
-    ∀ dst' idx' eₛ' eₜ' ς,
     dst' = dst.[ς] →
     idx' = idx.[ς] →
     eₛ' = eₛ.[ς] →
     eₜ' = eₜ.[ς] →
-    tmc_dps ξ dst' idx' eₛ' eₜ'
-  ).
-Proof.
-  apply tmc_ind; solve
-  [ intros; simplify; eauto with tmc
-  | intros * ? ? ? IHdps **; simplify;
-    econstructor; try naive_solver; try eapply IHdps with (up ς); autosubst
-  ].
-Qed.
-Lemma tmc_dir_subst ξ ς eₛ eₛ' eₜ eₜ' :
-  tmc_dir ξ eₛ eₜ →
-  eₛ' = eₛ.[ς] →
-  eₜ' = eₜ.[ς] →
-  tmc_dir ξ eₛ' eₜ'.
-Proof.
-  eauto using (proj1 (tmc_subst ξ)).
-Qed.
-Lemma tmc_dps_subst ξ ς dst dst' idx idx' eₛ eₛ' eₜ eₜ' :
-  tmc_dps ξ dst idx eₛ eₜ →
-  dst' = dst.[ς] →
-  idx' = idx.[ς] →
-  eₛ' = eₛ.[ς] →
-  eₜ' = eₜ.[ς] →
-  tmc_dps ξ dst' idx' eₛ' eₜ'.
-Proof.
-  eauto using (proj2 (tmc_subst ξ)).
-Qed.
+    tmc_dps ξ dst' idx' eₛ' eₜ'.
+  Proof.
+    eauto using (proj2 tmc_subst).
+  Qed.
 
-Section well_formed.
-  Context {progₛ progₜ} (tmc : tmc progₛ progₜ).
-
-  Lemma expr_well_formed_tmc :
+  Lemma expr_closed_tmc :
     ( ∀ eₛ eₜ,
-      tmc_dir tmc.(tmc_ξ) eₛ eₜ →
+      tmc_dir ξ eₛ eₜ →
       ∀ lvl,
-      expr_well_formed progₛ lvl eₛ →
-      expr_well_formed progₜ lvl eₜ
+      expr_closed lvl eₛ →
+      expr_closed lvl eₜ
     ) ∧ (
       ∀ dst idx eₛ eₜ,
-      tmc_dps tmc.(tmc_ξ) dst idx eₛ eₜ →
+      tmc_dps ξ dst idx eₛ eₜ →
       ∀ lvl,
-      expr_well_formed progₜ lvl dst →
-      expr_well_formed progₜ lvl idx →
-      expr_well_formed progₛ lvl eₛ →
-      expr_well_formed progₜ lvl eₜ
+      expr_closed lvl dst →
+      expr_closed lvl idx →
+      expr_closed lvl eₛ →
+      expr_closed lvl eₜ
     ).
   Proof.
     apply tmc_ind; try naive_solver.
-    - intros []; try done. intros lvl Hfuncₛ.
-      rewrite /= tmc.(tmc_dom). apply elem_of_union_l. done.
-    - intros * Hdir1 IH1 Hdps2 IH2 lvl (Hwf1 & Hwf2).
+    - intros * Hdir1 IH1 Hdps2 IH2 lvl (Hclosed1 & Hclosed2).
       simpl. split_and!; try naive_solver lia.
-      apply IH2; try naive_solver lia. apply expr_well_formed_lift1. done.
-    - intros * Hdir2 IH2 Hdps1 IH1 lvl (Hwf1 & Hwf2).
+      apply IH2; try naive_solver lia. apply expr_closed_lift1. done.
+    - intros * Hdir2 IH2 Hdps1 IH1 lvl (Hclosed1 & Hclosed2).
       simpl. split_and!; try naive_solver lia.
-      apply IH1; try naive_solver lia. apply expr_well_formed_lift1. done.
-    - intros * Hdir1 IH1 Hdps2 IH2 lvl Hdst_wf Hidx_wf (Hwf1 & Hwf2).
-      split; first auto. apply IH2; try done; apply expr_well_formed_lift1; done.
-    - intros * Hξ Hdir IH -> lvl Hdst_wf Hidx_wf (Hfuncₛ%lookup_lookup_total_dom & Hwf).
-      eapply (tmc.(tmc_dpss)) in Hfuncₛ as (eₜ' & Hfunc_dpsₜ & ?); last done.
+      apply IH1; try naive_solver lia. apply expr_closed_lift1. done.
+    - intros * Hdir1 IH1 Hdps2 IH2 lvl Hdst Hidx (Hclosed1 & Hclosed2).
+      split; first auto. apply IH2; try done; apply expr_closed_lift1; done.
+    - intros * Hξ Hdir IH -> lvl Hdst Hidx (_ & Hwf).
+      simpl. split_and!; [eauto using expr_closed_lift1.. | lia].
+    - intros * Hdir1 IH1 Hdps2 IH2 -> lvl Hdst Hidx (Hwf1 & Hwf2).
       simpl. split_and!; try naive_solver lia.
-      + eapply elem_of_dom_2. done.
-      + apply expr_well_formed_lift1. done.
-      + apply expr_well_formed_lift1. done.
-    - intros * Hdir1 IH1 Hdps2 IH2 -> lvl Hdst_wf Hidx_wf (Hwf1 & Hwf2).
+      + apply expr_closed_lift1. done.
+      + apply expr_closed_lift1. done.
+      + apply (expr_closed_le (S (S lvl))); first lia.
+        apply expr_closed_lift1, IH2; try naive_solver lia.
+        apply expr_closed_lift1. done.
+    - intros * Hdir2 IH2 Hdps1 IH1 -> lvl Hdst Hidx (Hwf1 & Hwf2).
       simpl. split_and!; try naive_solver lia.
-      + apply expr_well_formed_lift1. done.
-      + apply expr_well_formed_lift1. done.
-      + apply (expr_well_formed_le _ (S (S lvl))); first lia.
-        apply expr_well_formed_lift1, IH2; try naive_solver lia.
-        apply expr_well_formed_lift1. done.
-    - intros * Hdir2 IH2 Hdps1 IH1 -> lvl Hdst_wf Hidx_wf (Hwf1 & Hwf2).
-      simpl. split_and!; try naive_solver lia.
-      + apply expr_well_formed_lift1. done.
-      + apply expr_well_formed_lift1. done.
-      + apply (expr_well_formed_le _ (S (S lvl))); first lia.
-        apply expr_well_formed_lift1, IH1; try naive_solver lia.
-        apply expr_well_formed_lift1. done.
+      + apply expr_closed_lift1. done.
+      + apply expr_closed_lift1. done.
+      + apply (expr_closed_le (S (S lvl))); first lia.
+        apply expr_closed_lift1, IH1; try naive_solver lia.
+        apply expr_closed_lift1. done.
   Qed.
-  Lemma expr_well_formed_tmc_dir lvl eₛ eₜ :
-    tmc_dir tmc.(tmc_ξ) eₛ eₜ →
-    expr_well_formed progₛ lvl eₛ →
-    expr_well_formed progₜ lvl eₜ.
+  Lemma expr_closed_tmc_dir lvl eₛ eₜ :
+    tmc_dir ξ eₛ eₜ →
+    expr_closed lvl eₛ →
+    expr_closed lvl eₜ.
   Proof.
-    eauto using (proj1 (expr_well_formed_tmc)).
+    eauto using (proj1 expr_closed_tmc).
   Qed.
-  Lemma expr_well_formed_tmc_dps lvl dst idx eₛ eₜ :
-    tmc_dps tmc.(tmc_ξ) dst idx eₛ eₜ →
-    expr_well_formed progₜ lvl dst →
-    expr_well_formed progₜ lvl idx →
-    expr_well_formed progₛ lvl eₛ →
-    expr_well_formed progₜ lvl eₜ.
+  Lemma expr_closed_tmc_dps lvl dst idx eₛ eₜ :
+    tmc_dps ξ dst idx eₛ eₜ →
+    expr_closed lvl dst →
+    expr_closed lvl idx →
+    expr_closed lvl eₛ →
+    expr_closed lvl eₜ.
   Proof.
-    eauto using (proj2 (expr_well_formed_tmc)).
+    eauto using (proj2 expr_closed_tmc).
   Qed.
+End tmc.
 
-  Lemma program_well_formed_tmc :
-    program_well_formed progₛ →
-    program_well_formed progₜ.
-  Proof.
-    rewrite /program_well_formed !map_Forall_lookup => Hwf func eₜ Hfuncₜ.
-    apply elem_of_dom_2 in Hfuncₜ as Hfuncₜ'. rewrite tmc.(tmc_dom) elem_of_union in Hfuncₜ'.
-    destruct Hfuncₜ' as [Hfuncₛ%lookup_lookup_total_dom | (func_dir & Hξ)%elem_of_map_img].
-    - edestruct tmc.(tmc_dirs) as (_eₜ & Hdir & Heq); first done.
-      eapply expr_well_formed_tmc_dir; last naive_solver.
-      rewrite Heq in Hfuncₜ. naive_solver.
-    - pose proof Hξ as Hfunc_dirₛ%elem_of_dom_2%(tmc.(tmc_ξ_dom))%lookup_lookup_total_dom.
-      edestruct tmc.(tmc_dpss) as (eₜ' & Hdps & Heq); [done.. |].
-      rewrite Hfuncₜ in Heq. injection Heq as ->.
-      repeat constructor. eapply expr_well_formed_tmc_dps; [naive_solver.. |].
-      apply (expr_well_formed_le _ 1); naive_solver lia.
-  Qed.
-End well_formed.
+#[export] Hint Resolve tmc_dir_refl : tmc.
+
+Lemma program_closed_tmc progₛ progₜ :
+  tmc progₛ progₜ →
+  program_closed progₛ →
+  program_closed progₜ.
+Proof.
+  intros tmc. rewrite /program_closed !map_Forall_lookup => Hclosed func eₜ Hfuncₜ.
+  apply elem_of_dom_2 in Hfuncₜ as Hfuncₜ'. rewrite tmc.(tmc_dom) elem_of_union in Hfuncₜ'.
+  destruct Hfuncₜ' as [Hfuncₛ%lookup_lookup_total_dom | (func_dir & Hξ)%elem_of_map_img].
+  - edestruct tmc.(tmc_dirs) as (_eₜ & Hdir & Heq); first done.
+    eapply expr_closed_tmc_dir; last naive_solver.
+    rewrite Heq in Hfuncₜ. naive_solver.
+  - pose proof Hξ as Hfunc_dirₛ%elem_of_dom_2%(tmc.(tmc_ξ_dom))%lookup_lookup_total_dom.
+    edestruct tmc.(tmc_dpss) as (eₜ' & Hdps & Heq); [done.. |].
+    rewrite Hfuncₜ in Heq. injection Heq as ->.
+    repeat constructor. eapply expr_closed_tmc_dps; [naive_solver.. |].
+    apply (expr_closed_le 1); naive_solver lia.
+Qed.
